\section{Stability Estimates for Pyramidal Finite Elements} % (fold)
\label{sec:pyramidal_finite_elements}
$\hat{E}$ will be the reference pyramid  in Figure~\ref{reference_pyramid}.
Anisotropic interpolation error estimates for pyramidal $\bcurl$--conforming
and div--conforming finite elements of least order will we established.
\begin{lemma}\label{auxlabel350}
  The shape functions in Tables~\ref{shape_edge_table} and~\ref{shape_face_table}
  are bounded.
\end{lemma}
\begin{proof}
  Observe that the pyramid is contained in the region $\{\,x+z\leqslant 1,\,y+z\leqslant 1\,\}$
  which yields
  \begin{IEEEeqnarray*}{rClcrClcrCl}
    \tfrac{x}{1-z}&\leqslant& 1\mbox{,} &\quad&
    \tfrac{xy}{1-z}&\leqslant& y\mbox{,}&\quad&
    \tfrac{xyz}{(1-z)^2}&\leqslant& z.
  \end{IEEEeqnarray*}
\end{proof}
\subsection{Anisotropic Stability Estimates for $H(\bcurl)$--Conforming 
Elements on Pyramids} % (fold)
\label{sub:edge_elements}
\input{./chap_additional/stability_edge_ref_pyramid}
% subsection edge_elements (end)
\subsection{Anisotropic Stability Estimates for $H(\text{div})$--Conforming 
Elements on Pyramids} % (fold)
\label{sub:face_elements}
Here we will work on the div--conforming analogue of
Theorem~\ref{aux_label53}.
\begin{theorem} \label{aux_label54}
Let $\hat E$ be the reference pyramid and let $p>1$. Let $\br_{\hat E}(\cdot)$ denote
the interpolation operator determined by the degrees of freedom in Definition~\ref{aux_label71}.
There is $C>0$ such that,
for all $\hat\bu\in W^{1,p}(\hat E)$, there hold
\begin{IEEEeqnarray*}{rCl}
  \|(\rku)_1\|_{\scriptscriptstyle{L^\infty(\hat{E})}}
  &\lesssim& \|\hat u_1\|_{\scriptscriptstyle{W^{1,1}(\hat{E})}} +
    \|\dv \hat\bu\|_{\scriptscriptstyle{L^1}(\hat{E})} + 
    \left\|\hat{u}_3\right\|_{\scriptscriptstyle{W^{1,1}}(\hat{E})}\\[12pt]
  \|(\rku)_2\|_{\scriptscriptstyle{L^\infty(\hat{E})}}
  &\lesssim& \|\hat u_2\|_{\scriptscriptstyle{W^{1,1}(\hat{E})}} +
    \|\dv \hat\bu\|_{\scriptscriptstyle{L^1}(\hat{E})} + 
    \left\|\hat{u}_3\right\|_{\scriptscriptstyle{W^{1,1}}(\hat{E})}\\[12pt]
  \|(\rku)_3\|_{\scriptscriptstyle{L^\infty(\hat{E})}} & \lesssim & 
    \|\hat u_3\|_{\scriptscriptstyle{W^{1,1}(\hat{E})}} +
    \|\dv \hat\bu\|_{\scriptscriptstyle{L^1}(\hat{E})}.
\end{IEEEeqnarray*}
\end{theorem}
\begin{proof}
We will use the notation of Table~\ref{shape_face_table} for the 
shape functions and Tables~\ref{pyramidNotationTableFaces} and~\ref{pyramidNotationTableEdges}
for the boundary of the reference pyramid. This proof is based on explicit computation as well.
The variables 
in the local coordinate system of $\hat E$ for the shape functions $\hat\bz_i$ 
are $x$, $y$ and $z$ instead
of $\hat x_1$, $\hat x_2$ and $\hat x_3$.\\[5pt]
Consider the case $\hat{\bu} = (\hat{u}_1,0,0)'$ to start with and compute it's 
interpolate. 
\begin{IEEEeqnarray*}{rCl}
  \rku & = & \{{\scriptstyle\iint_{\hat{f}_2} \hat\bu \cdot \hat\bn_2\,d\hat S}\}\,\hat\bz_2 + 
             \{{\scriptstyle\iint_{\hat{f}_3} \hat\bu \cdot \hat\bn_3\,d\hat S}\}\,\hat\bz_3\\[4pt]
       & =: & \rho_2(\hat\bu)\,\hat\bz_2 + \rho_3(\hat\bu)\,\hat\bz_3.
\end{IEEEeqnarray*}
Then for the first two components of the interpolate it holds
\begin{IEEEeqnarray*}{rCl}
  (\rku)_1(x,y,z) & = & -2\rho_2(\hat\bu) + 
    \{\rho_2(\hat\bu)+\rho_3(\hat\bu)\}\,\tfrac{2x-xz}{1-z}\\[4pt]
    & = & -2{\iint_{\hat{f}_2} \hat{\bu} \cdot \hat\bn_2\,d\hat S}\\[4pt]
    &&\, +\,\left\{
          {\iint_{\hat{f}_2} \hat{\bu} \cdot \hat\bn_2\,d\hat S}+
                  {\iint_{\hat{f}_3} \hat{\bu} \cdot \hat\bn_3\,d\hat S}\right\}
                  \tfrac{2x-xz}{1-z}\\[4pt]
    & = & -2{\iint_{\hat{f}_2} \hat{\bu} \cdot \hat\bn_2\,d\hat S} + 
          {\iint_{\partial\hat{E}} \hat{\bu} \cdot \hat\bn\,d\hat S}\,\tfrac{2x-xz}{1-z}\\[4pt]
    & = & -2{\iint_{\hat{f}_2} \hat{\bu} \cdot \hat\bn_2\,d\hat S} + 
            {\int_{\hat{E}} \dv\hat{\bu} \,d\hat{\boldsymbol{x}}}\,\tfrac{2x-xz}{1-z}
\end{IEEEeqnarray*}
and
\begin{IEEEeqnarray*}{rCl}
  (\rku)_2\xyz & = & -(\rho_2(\hat\bu)+\rho_3(\hat\bu))\,\tfrac{yz}{1-z}\\[4pt]
    & = & -{\int_{\hat{E}} \dv\hat{\bu} \,d\hat{\boldsymbol{x}}}\,\tfrac{yz}{1-z}.
\end{IEEEeqnarray*}
Switch to $\hat{\bu}$ of the form $(0,\hat{u}_2,0)'$.
\begin{IEEEeqnarray*}{rCl}
  \rku & = & ({\scriptstyle\iint_{\hat{f}_1} \hat\bu \cdot \hat\bn_1\,d\hat S})\,\hat\bz_1 + 
         ({\scriptstyle\iint_{\hat{f}_4} \hat\bu \cdot \hat\bn_4\,d\hat S})\,\hat\bz_4\\[4pt]
       & = & \rho_1(\hat\bu)\,\hat\bz_1 + \rho_4(\hat\bu)\,\hat\bz_4.
\end{IEEEeqnarray*}
Then summing up yields, for now,
\begin{IEEEeqnarray*}{rCl}
  (\rku)_1(x,y,z) & = & -(\rho_1(\hat\bu)+\rho_4(\hat\bu))\,\tfrac{xz}{1-z}\\[4pt]
    & = & -{\int_{\hat{E}} \dv\hat{\bu} \,d\hat{\boldsymbol{x}}}\,\tfrac{xz}{1-z}.\\[8pt]
  (\rku)_2(x,y,z) & = & -2\rho_1(\hat\bu) + 
  (\rho_1(\hat\bu)+\rho_4(\hat\bu))\,\tfrac{2y-yz}{1-z}\\[4pt]
    & = & -2{\iint_{\hat{f}_1} \hat{\bu} \cdot \hat\bn_1\,d\hat S} + 
            {\iint_{\partial\hat{E}} \hat{\bu} \cdot \hat\bn\,d\hat S}\,\tfrac{2y-yz}{1-z}\\[4pt]
    & = & -2{\iint_{\hat{f}_1} \hat{\bu} \cdot \hat\bn_1\,d\hat S} + 
            {\int_{\hat{E}} \dv\hat{\bu} \,d\hat{\boldsymbol{x}}}\,\tfrac{2y-yz}{1-z}.\\[8pt]
\end{IEEEeqnarray*}
Now continue with $\hat{\bu}$ of the form $(0,0,\hat{u}_3)'$.
\begin{IEEEeqnarray*}{rCl}
  \rku & = & ({\scriptstyle\iint_{\hat{f}_3} \hat\bu \cdot \hat\bn_3\,d\hat S})\,\hat\bz_3 + 
         ({\scriptstyle\iint_{\hat{f}_4} \hat\bu \cdot \hat\bn_4\,d\hat S})\,\hat\bz_4 + 
         ({\scriptstyle\iint_{\hat{f}_5} \hat\bu \cdot \hat\bn_5\,d\hat S})\,\hat\bz_5\\[4pt]
       & =: & \rho_3(\hat\bu)\,\hat\bz_3 + \rho_4(\hat\bu)\,\hat\bz_4
       + \rho_5(\hat\bu)\,\hat\bz_5.
\end{IEEEeqnarray*}
Then
\begin{IEEEeqnarray*}{rCl}
  (\rku)_1(x,y,z) & = & \{\rho_3(\hat\bu) + \rho_5(\hat\bu)\}\,x
  + \rho_3(\hat\bu) \tfrac{x}{1-z} - \rho_4\tfrac{xz}{1-z}.
\end{IEEEeqnarray*}
Now observe that
\begin{IEEEeqnarray*}{rCl}
  (\rho_3 + \rho_5)(\hat\bu) & = & 
    {\iint_{\partial\hat{E}} \hat{\bu} \cdot \hat\bn\,d\hat S} - 
      {\iint_{\hat{f}_4} \hat{\bu} \cdot \hat\bn_4\,d\hat S} \\[4pt]
  & = & {\int_{\hat{E}} \dv\hat{\bu}\,d\hat{\boldsymbol{x}}} - 
        \rho_4(\hat{\bu})
\end{IEEEeqnarray*}
and, on the other hand,
\begin{IEEEeqnarray*}{rCl}
  (\rho_3-\rho_4)(\hat\bu) & = & 
  {\iint_{\hat{f}_3} \hat\bu \cdot \hat\bn_3\,d\hat S} - 
  {\iint_{\hat{f}_4} \hat\bu \cdot \hat\bn_4\,d\hat S} \\[4pt]
  & = & \int_{0}^{1}\int_{0}^{x} \hat{u}_3(x,y,1-x)\,dydx - 
        \int_{0}^{1}\int_{0}^{y} \hat{u}_3(x,y,1-y)\,dxdy\mbox{,}
\end{IEEEeqnarray*}
so
\begin{IEEEeqnarray*}{rCl}
  (\rku)_1(x,y,z) & = & {x\int_{\hat{E}} \dv\hat{\bu}\,d\hat{\boldsymbol{x}}}\,+\\[4pt]
  \IEEEeqnarraymulticol{3}{r}{
    \qquad\left\{\int_{0}^{1}\int_{0}^{x} \hat{u}_3(x,y,1-x)\,dydx - 
    \int_{0}^{1}\int_{0}^{y} \hat{u}_3(x,y,1-y)\,dxdy\right\}\,
    \tfrac{x}{1-z}.}
\end{IEEEeqnarray*}
In a completely similar fashion we arrive at
\begin{IEEEeqnarray*}{rCl}
  (\rku)_2(x,y,z) & = & y\,{\int_{\hat{E}} \dv\hat{\bu}\,d\hat{\boldsymbol{x}}}\,+
  \left\{{\iint_{\hat{f}_3} \hat\bu \cdot \hat\bn_3\,d\hat S} - 
   {\iint_{\hat{f}_4} \hat\bu \cdot \hat\bn_4\,d\hat S}\right\}\,\tfrac{y}{1-z}.\\[4pt]
               & = & y\,{\int_{\hat{E}} \dv\hat{\bu}\,d\hat{\boldsymbol{x}}}\,+\\[4pt]
  \IEEEeqnarraymulticol{3}{r}{
    \qquad\left\{\int_{0}^{1}\int_{0}^{x} \hat{u}_3(x,y,1-x)\,dydx - 
    \int_{0}^{1}\int_{0}^{y} \hat{u}_3(x,y,1-y)\,dxdy\right\}
    \tfrac{y}{1-z}.}
\end{IEEEeqnarray*}
We collect every term obtained so far for the first and second components in
Table~\ref{terms_table}.
\begin{table}[!h]
    \centering  
    \caption{Terms\\[4pt]$q(s,t) = \tfrac{2s-st}{1-t},\,r(s,t) = \tfrac{st}{1-t}$}
    \label{terms_table}
    \begin{IEEEeqnarraybox*}
    [\IEEEeqnarraystrutmode
    \IEEEeqnarraystrutsizeadd{2pt}{12pt}]{v/c/v/c/v/c/v/}
        \IEEEeqnarrayrulerow\\
        \IEEEeqnarrayseprow[5pt]\\
        & & & (\rku)_1 & & (\rku)_2 & \\
        \IEEEeqnarrayrulerow\\
        \IEEEeqnarrayseprow[5pt]\\
        & (\hat{u}_1,0,0)' & &
          \begin{IEEEeqnarraybox*}{l}
            -2{\iint_{\hat{f}_2} \hat{\bu} \cdot \hat\bn_2\,d\hat S}\\ + 
            {q(x,z)\int_{\hat{E}} \dv\hat{\bu} \,d\hat{\boldsymbol{x}}}
          \end{IEEEeqnarraybox*}
        & &
          -r(y,z){\int_{\hat{E}} \dv\hat{\bu} \,d\hat{\boldsymbol{x}}} &\\
        \IEEEeqnarrayrulerow\\
        \IEEEeqnarrayseprow[5pt]\\
        & (0,\hat{u}_2,0)' & & 
          -r(x,z){\int_{\hat{E}} \dv\hat{\bu} \,d\hat{\boldsymbol{x}}} 
        & & 
          \begin{IEEEeqnarraybox*}{l}
            -2{\iint_{\hat{f}_1} \hat{\bu} \cdot \hat\bn_1\,d\hat S}\\ + 
            {q(x,z)\int_{\hat{E}} \dv\hat{\bu} \,d\hat{\boldsymbol{x}}}
          \end{IEEEeqnarraybox*}
        &\\
        \IEEEeqnarrayrulerow\\
        \IEEEeqnarrayseprow[5pt]\\
        & (0,0,\hat{u}_3)' & & 
          \begin{IEEEeqnarraybox*}{l}
            x\int_{\hat{E}} \dv\hat{\bu}\,d\hat{\boldsymbol{x}} \\[5pt] +\, 
            \left\{\iint_{\hat{f}_3} \hat\bu \cdot \hat\bn_3\,d\hat S\right.
             \\[5pt] 
            \left. -\iint_{\hat{f}_4} \hat\bu \cdot \hat\bn_4\,d\hat S\right\}r(x,z)
          \end{IEEEeqnarraybox*}
         & & 
          \begin{IEEEeqnarraybox*}{l}
            y\int_{\hat{E}} \dv\hat{\bu}\,d\hat{\boldsymbol{x}}\\[5pt] +\, 
              \left\{\iint_{\hat{f}_4} \hat\bu \cdot \hat\bn_4\,d\hat S\right.
             \\[5pt] 
             \left.-\iint_{\hat{f}_3} \hat\bu \cdot \hat\bn_3\,d\hat S\right\}r(y,z)
          \end{IEEEeqnarraybox*}
        &\\\IEEEeqnarrayrulerow
    \end{IEEEeqnarraybox*}
\end{table}

Lastly, the third component of $\rku$ can be treated at once for any 
field $\hat\bu$ as follows:
\begin{IEEEeqnarray*}{rCl}
    (\rku)_3(x,y,z) & = &   z\sum_{i=1}^4\iint_{\hat{f}_i} \hat{\bu}\cdot\hat{\bn}_i\,d\hat S
                      + (z-1) \iint_{\hat{f}_5}\hat{\bu}\cdot\hat{\bn}_5\,d\hat S\\[5pt]
                    & = & z\iint_{\partial\hat{E}} \hat{\bu}\cdot\hat{\bn} - \iint_{f_5}
                 \hat{\bu}\cdot\hat{\bn}_5\,d\hat S\\[5pt]
    \yesnumber\label{term_rk3}
                    & = &\hat{x}_3\int_{\hat{E}} \mbox{div}\,\hat{\bu}\,d\hat{\bx} 
     + \iint_{\hat{f}_5} \hat{u}_3\,d\hat{S}.
\end{IEEEeqnarray*}
Now we bound each term in Table~\ref{terms_table} and in expression~(\ref{term_rk3}).
\begin{IEEEeqnarray*}{rCl}
  (\rku)_1 & = & (\br_{\hat{E}}(\hat{u}_1,0,0)')_1 + 
                 (\br_{\hat{E}}(0,\hat{u}_2,0)')_1 + 
                 (\br_{\hat{E}}(0,0,\hat{u}_3)')_1\\[5pt]
           & = & -2\iint_{\hat{f}_2}\hat{u}_1\,d\hat S +
  \tfrac{2x}{1-z}\int_{\hat{E}} \tfrac{\partial\hat{u}_1}{\partial\hat{x}_1}\,d\hat{\bx} -
  \tfrac{xz}{1-z}\int_{\hat{E}} \tfrac{\partial\hat{u}_1}{\partial\hat{x}_1}\,d\hat{\bx} \\[5pt]
  & & \,- \tfrac{xz}{1-z}\int_{\hat{E}} \tfrac{\partial\hat{u}_2}{\partial\hat{x}_2}\,d\hat{\bx}
  + \left( x + \tfrac{xz}{1-z}-\tfrac{xz}{1-z} \right)
  \int_{\hat{E}} \tfrac{\partial\hat{u}_3}{\partial\hat{x}_3}\,d\hat{\bx}\\[5pt]
  &   &\, + \left({\iint_{\hat{f}_3} \hat{u}_3\,d\hat S}
        - {\iint_{\hat{f}_4} \hat{u}_3\,d\hat S}\right)\tfrac{xz}{1-z}\\[5pt]
           & = & -2\iint_{\hat{f}_2}\hat{u}_1\,d\hat S +
  \tfrac{2x}{1-z}\int_{\hat{E}}\tfrac{\partial\hat{u}_1}{\partial\hat{x}_1}\,d\hat{\bx} -
  \tfrac{xz}{1-z}\int_{\hat{E}}\dv\hat{\bu}\,d\hat{\bx}\\[5pt]
  \yesnumber\label{face_integrals}
  &  & \,+\tfrac{x}{1-z}\int_{\hat{E}}\tfrac{\partial\hat{u}_3}{\partial\hat{x}_3}\,d\hat{\bx}
  + \left({\iint_{\hat{f}_3} \hat{u}_3\,d\hat S}
        - {\iint_{\hat{f}_4} \hat{u}_3\,d\hat S}\right)\tfrac{xz}{1-z}.
\end{IEEEeqnarray*}
For the surface integrals in~(\ref{face_integrals}), by Lemma 5.15 in~\cite{monk}, page 120,
\begin{IEEEeqnarray*}{rCl}
\left|\iint_{\hat{f}_2} \hat{u}_1\,d\hat S\right| 
  & \leqslant & C\,\|\hat{u}_1\|_{H^{1}(\hat{E})}
\end{IEEEeqnarray*}
and similarly
\begin{IEEEeqnarray*}{rCl}
  \left|\iint_{\hat{f}_3} \hat{u}_3\,d\hat S - \iint_{\hat{f}_4} \hat{u}_3\,d\hat S\right| 
  & \leqslant & C\,\|\hat{u}_3\|_{H^{1}(\hat{E})}
\end{IEEEeqnarray*}
all of which, together with Lemma~\ref{auxlabel350}, leads to
\begin{IEEEeqnarray*}{rCl}
  \|(\rku)_1\|_{L^{\infty}(\hat{E})} & \leqslant & C_{\hat{E}} 
  \left[ 
    \|\hat{u}_1\|_{H^{1}(\hat{E})} + 
    \|\dv\hat{\bu}\|_{L^{1}(\hat{E})} + 
    \|\hat{u}_3\|_{H^{1}(\hat{E})}
  \right].
\end{IEEEeqnarray*}
Copying the argument for the second component
\begin{IEEEeqnarray*}{rCl}
  \|(\rku)_2\|_{L^{\infty}(\hat{E})} & \leqslant & C_{\hat{E}} 
  \left[ 
    \|\hat{u}_2\|_{H^{1}(\hat{E})} + 
    \|\dv\hat{\bu}\|_{L^{1}(\hat{E})} + 
    \|\hat{u}_3\|_{H^{1}(\hat{E})}
  \right].
\end{IEEEeqnarray*}
Finally from~(\ref{term_rk3}) we deduce
\begin{IEEEeqnarray*}{rCl}
  \|(\rku)_3\|_{\scriptscriptstyle{L^\infty(\hat{E})}} & \leqslant & C_{\hat{E}}
    \left[\|\hat u_3\|_{\scriptscriptstyle{H^{1}(\hat{E})}} +
    \|\dv \hat\bu\|_{\scriptscriptstyle{L^1}(\hat{E})}\right].
\end{IEEEeqnarray*}
The quantity $C_{\hat{E}}$ depends only on the supremum of the (fixed)
basis shape functions of Table~\ref{shape_face_table} over the pyramid.
\end{proof}
{\color {red}SEGUIR ACA completar el enunciado}\\\\
The next result is the div--conforming analogue of Theorem~\ref{auxlabel211},
\begin{theorem}
Let $E$ be any pyramid which is
  a non degenerate affine image 
  of the reference pyramid $\hat{E}$. We fix a positively oriented local system of 
  coordinates $(\bxi_1, \bxi_2, \bxi_3)$
  with origin in a vertex $\bx_E$ of the parallelogram basis, for which $(\bxi_1, \bxi_2)$
  correspond to the two basis edges incident to $\bx_E$ and $\bxi_3$ is parallel to the 
  edge joining $\bx_E$ with the top of the pyramid. Let $h_1, h_2, h_3$ be the corresponding 
  edge lengths. With $\partial^{\balpha}$ we denote 
  $\tfrac{\partial^{|\balpha|}}{\partial_{\bxi_1}^{\alpha_1}\partial_{\bxi_2}^{\alpha_2}\partial_{\bxi_3}^{\alpha_3}}$.
  For all $\bu\in W^{1,1}(E)^3$
\begin{IEEEeqnarray}{C}\nonumber
  \|\bu-\br_E \bu\|_{L^p(E)} \lesssim 
  \sum_{|{\balpha}|=1}\bh^{\balpha} \|\partial^{\balpha}\bu\|_{L^p(E)} +
  h_E\|\dv\bu\|_{L^p(E)}\\[4pt]
  \,+\, diff de u3 \\[4pt].
  \label{auxlabel214}
\end{IEEEeqnarray}
\end{theorem}
\begin{proof}
  Using~\eqref{pull1} again, using~\eqref{derivadaPiola} and repeating the steps 
  for~\eqref{auxlabel212}
  \begin{IEEEeqnarray*}{rCl}
    \|(\br_{\tilde{E}}\tilde{\bu})_1\|_{\scriptscriptstyle L^\infty(\tilde E)} &\lesssim& 
    \tfrac{1}{|\tilde E|} 
    \big\{
      \|\tilde{u}_1\|_{\scriptscriptstyle L^1(\tilde E)} + 
      \sum_i h_i\|\partial_{\tilde{x}_i}\tilde{u}_1\|_{\scriptscriptstyle L^1(\tilde E)} + 
      h_1\|\dv \tilde{\bu}\|_{\scriptscriptstyle L^1(\tilde E)} \\[5pt]
    \IEEEeqnarraymulticol{3}{r}{\,+\, 
      \|\tilde{u}_3\|_{\scriptscriptstyle L^1(\tilde E)} + 
      h_1\|\partial_{\tilde{x}_1}\tilde{u}_3\|_{\scriptscriptstyle L^1(\tilde E)} +
      h_2\|\partial_{\tilde{x}_2}\tilde{u}_3\|_{\scriptscriptstyle L^1(\tilde E)} + 
      h_1\|\partial_{\tilde{x}_3}\tilde{u}_3\|_{\scriptscriptstyle L^1(\tilde E)} 
     \big\}}
  \end{IEEEeqnarray*}
  The procedure for the second component is the same and the resulting estimate
  is symmetrical. For component three, the same procedure (with fewer terms) yields
  \begin{IEEEeqnarray*}{rCl}
  \|(\br_{\tilde{E}}\tilde{\bu})_3\|_{\scriptscriptstyle L^\infty(\tilde E)} &\lesssim& 
  |\tilde{E}|^{-1}\left(
  \|\tilde{u}_3\|_{\scriptscriptstyle L^1(\tilde{E})}
  +\sum_{i=1}^3h_i\|\partial_{\tilde{x}_i}\tilde{u}_3\|_{\scriptscriptstyle L^1(\tilde{E})}
  +h_3\|\dv \tilde{\bu} \|_{\scriptscriptstyle L^1(\tilde{E})}\right).
  \end{IEEEeqnarray*}
  applying \eqref{auxlabel213} and its analogue for the $L^\infty$ norm
  we sum the component estimates to obtain the vectorial stability estimate in a physical pyramid:
  \begin{IEEEeqnarray*}{rCl}
    \|\br_{\tilde E}\tilde\bu\|_{\scriptscriptstyle L^p(\tilde E)}& \lesssim &\\[5pt]
    \IEEEeqnarraymulticol{3}{r}{\|\tilde{\bu}\|_{\scriptscriptstyle L^p(\tilde E)} +
          \sum_i h_i\|\partial_{\tilde{x}_i}\tilde{\bu}\|_{\scriptscriptstyle L^p(\tilde E)} +
        h_{\tilde E}\|\dv \tilde\bu\|_{\scriptscriptstyle{L^p}(\tilde{E})} + 
        \max\{h_1,h_2\} \|D\tilde{u}_3\|_{\scriptscriptstyle L^p(\tilde E)}}.
  \end{IEEEeqnarray*}
Now we apply~\eqref{aux_label23} and~\eqref{aux_label30}
to the rescaled pyramid (Figure~\ref{rescaled_pyramid}), making use of the
approximation property for these finite elements
(see Section 5 of~\cite{gh99}), and 
continue as in Theorem~\ref{aux_label46} or~\ref{aux_label32} and the result
follows.
\end{proof}


% subsection face_elements (end)

%% TODO =======================================================================
%% poner tres dibujos con casos $h1=h2<h3$; $h1<h2<h3$; $h2<h1<h3$
% subsection local_interpolation_estimates_for_pyramidal_elements (end)
%% ============================================================================


% section pyramidal_finite_elements (end)