\section{Statement of the Main Approximation Error Theorem}
Recall from inequality~(\ref{aux_label48})  for every $\bw\in W(\Th)$ it holds
\begin{IEEEeqnarray*}{rCl}
  \|\bu-\bu_h\|_{L^2(\Omega)^3} &\leqslant& C\{\|\bu-\br_0\bu\|_{L^2(\Omega)^3} + \|\bu-\bw\|_{L^2(\Omega)^3}\}.
\end{IEEEeqnarray*}
For each $\bw$ we decompose the norm with the macro--elements as follows
\begin{IEEEeqnarray*}{rCl}
  \|\bu-\bw\|^2_{0,\Omega} &=& \sum_1^{N_{\textit{h}_0}} \|\bu-\bw\|^2_{0,\Lambda_\ell}\\
    &=& \sum_1^{N_{\textit{h}_0}} \left\{
      \sum_{pri} \|\bu-\bw\|^2_{0,E_\ell} +
      \sum_{tet} \|\bu-\bw\|^2_{0,E_\ell} +
      \sum_{pyr} \|\bu-\bw\|^2_{0,E_\ell}
    \right\} 
\end{IEEEeqnarray*}
%%=========================================================================
%For each macro--element $\Lambda_\ell$, for each pyramid $E_\ell\in\Lambda_\ell$,
%\begin{IEEEeqnarray*}{rCl}
%  \|\bu_s - \pi\bu_s\|^2_{\sss L^2(E)}&\leqslant&
%  h_1^2\|\gancho_{\xi_1}\bu_s\|^2+
%  h_2^2\|\gancho_{\eta_2}\bu_s\|^2+
%  h_3^2\|\gancho_{\xi_3}\bu_s\|^2+
%  h_K^2\|\dvg\bu_s\|^2\\[7pt]
%\end{IEEEeqnarray*}
%\begin{IEEEeqnarray*}{rCl}
%  h_1\|\gancho_{\xi_1}\bu_s\|&=&
%  h_1\sum_{i=1}^3 \|\gancho_{\xi_1}\bu_{s,i}\|\\
%  &\leqslant&
%    \textit{h}\sum_{i=1}^3 \|r^{1-\mu}\gancho_{\xi_1}\bu_{s,i}\|\\
%  &\leqslant&
%    \textit{h}\left(
%     \sum_{i=1}^2 \|R^{1-\mu}\theta^{1-\mu}\gancho_{\xi_1}\bu_{s,i}\|+
%     \|R^{1-\mu}\gancho_{\xi_1}\bu_{s,3}\|\right)\\[7pt]
%  &\leqslant&
%    \textit{h}\left(
%     \sum_{i=1}^2 \|R^{1-\nu}\theta^{1-\mu}\gancho_{\xi_1}\textbf{u}_{s,i}\|+
%     \|R^{1-\nu}\gancho_{\xi_1}\textbf{u}_{s,3}\|\right)\\[7pt]
%  &\leqslant&
%    \textit{h}\left(
%    \sum_{i=1}^2 \|R^{\beta}\theta^{\delta}\gancho_{\xi_1}\textbf{u}_{s,i}\|+
%     \|R^{\beta}\gancho_{\xi_1}\textbf{u}_{s,3}\|\right)\\[7pt]
%  &\leqslant&
%    \textit{h}
%    \left(\sum_{i=1}^2 \|\textbf{u}_{s,i}\|_{\scriptscriptstyle \beta,\delta}+
%         \|\textbf{u}_{s,3}\|_{\scriptscriptstyle \beta,0}\right).
%\end{IEEEeqnarray*}
%%=========================================================================
Take $\bw_{\bu}$ as in Definition~\ref{aux_label51}.
For the sum term over the pyramids (remember pyramids do not touch singularities)
we have, restricting $\bw_{\bu}$, by the inequality we proved in~(\ref{aux_label63})  for pyramids
\begin{IEEEeqnarray*}{rCl}
  \|\bu-\bw_{\bu}\|^2_{0,E_\ell} & = & \|\bu-P_{0,E_{\ell}}\bu\|^2_{0,E_\ell}\\
                           & \leqslant & C \left\{h_E|\bu_r|_{H^1(E_\ell)} 
                                + h_E|\bu_s|_{H^1(E_\ell)}\right\}\\
                           & \leqslant & C\textit{h}\left\{ |\bu_r|_{H^1(E)} 
                              + \|\bu_s\|_{V^{1,2}_{\beta,\delta}(E)}\right\}.
\end{IEEEeqnarray*}
With this all the others for prisms and tetrahedra whithin the proof of the
interpolation Theorem~\ref{interpolation_theorem} we have
\begin{IEEEeqnarray*}{rCl}
  \|\bu-\bw_{\bu}\|^2_{0,\Omega}
    &=& \sum_{\ell=1}^{N_{\textit{h}_0}} \left\{
      \sum_{pri} \|\bu-\br_0\bu\|^2_{0,E_\ell} +
      \sum_{tet} \|\bu-\br_0\bu\|^2_{0,E_\ell} +
      \sum_{pyr} \|\bu-P_{0,E_{\ell}}\bu\|^2_{0,E_\ell}
    \right\}\\[5pt]
    &\leqslant& C \sum_{\ell=1}^{N_{\textit{h}_0}}
      \textit{h}^2 \|f\|^2_{0,\Omega}\\[5pt]
\yesnumber\label{aux_label62}
    & \leqslant &  C\,\textit{h}^2 \|f\|^2_{0,\Omega}.
\end{IEEEeqnarray*}
Note $C$ depends on the cardinal of the initial mesh.
Now by Theorem~\ref{interpolation_theorem} and~(\ref{aux_label62}) we have, for 
the vectorial variable, 
$\|\bu-\bu_h\|_{L^2(\Omega)^3} \leqslant C\textit{h}\|f\|_{L^2(\Omega)}$.
